finished: implement lazy and force

erasure/theories/EImplementLazuForce.v
@@ -24,36 +24,35 @@ Hint Constructors eval : core.
 
 Import MCList (map_InP, map_InP_elim, map_InP_spec).
 
-Section implement_thunk.
+Section implement_lazy_force.
   Context (Σ : global_declarations).
 
   Section Def.
 
-  Equations? implement_thunk (t : term) : term
+  Equations? implement_lazy_force (t : term) : term
     by wf t (fun x y : EAst.term => size x < size y) :=
     | tRel i => EAst.tRel i
-    | tEvar ev args => EAst.tEvar ev (map_InP args (fun x H => implement_thunk x))
-    | tLambda na M => EAst.tLambda na (implement_thunk M)
-    | tApp u v := tApp (implement_thunk u) (implement_thunk v)
-    | tLetIn na b b' => EAst.tLetIn na (implement_thunk b) (implement_thunk b')
+    | tEvar ev args => EAst.tEvar ev (map_InP args (fun x H => implement_lazy_force x))
+    | tLambda na M => EAst.tLambda na (implement_lazy_force M)
+    | tApp u v := tApp (implement_lazy_force u) (implement_lazy_force v)
+    | tLetIn na b b' => EAst.tLetIn na (implement_lazy_force b) (implement_lazy_force b')
     | tCase ind c brs =>
-      let brs' := map_InP brs (fun x H => (x.1, lift 1 #|x.1| (implement_thunk x.2))) in
-      EAst.tLetIn (nNamed "discr") (implement_thunk c)
-      (EAst.tCase (ind.1, 0) (tRel 0) brs')
-    | tProj p c => EAst.tProj {| proj_ind := p.(proj_ind); proj_npars := 0; proj_arg := p.(proj_arg) |} (implement_thunk c)
+      let brs' := map_InP brs (fun x H => (x.1, (implement_lazy_force x.2))) in
+      (EAst.tCase (ind.1, 0) (implement_lazy_force c) brs')
+    | tProj p c => EAst.tProj {| proj_ind := p.(proj_ind); proj_npars := 0; proj_arg := p.(proj_arg) |} (implement_lazy_force c)
     | tFix mfix idx =>
-      let mfix' := map_InP mfix (fun d H => {| dname := dname d; dbody := implement_thunk d.(dbody); rarg := d.(rarg) |}) in
+      let mfix' := map_InP mfix (fun d H => {| dname := dname d; dbody := implement_lazy_force d.(dbody); rarg := d.(rarg) |}) in
       EAst.tFix mfix' idx
     | tCoFix mfix idx =>
-      let mfix' := map_InP mfix (fun d H => {| dname := dname d; dbody := implement_thunk d.(dbody); rarg := d.(rarg) |}) in
+      let mfix' := map_InP mfix (fun d H => {| dname := dname d; dbody := implement_lazy_force d.(dbody); rarg := d.(rarg) |}) in
       EAst.tCoFix mfix' idx
     | tBox => tBox
     | tVar n => EAst.tVar n
     | tConst n => EAst.tConst n
-    | tConstruct ind i block_args => EAst.tConstruct ind i (map_InP block_args (fun d H => implement_thunk d))
-    | tPrim p => EAst.tPrim (map_primIn p (fun x H => implement_thunk x))
-    | tLazy t => EAst.tLambda nAnon (lift 1 0 (implement_thunk t))
-    | tForce t => EAst.tApp (implement_thunk t) tBox.
+    | tConstruct ind i block_args => EAst.tConstruct ind i (map_InP block_args (fun d H => implement_lazy_force d))
+    | tPrim p => EAst.tPrim (map_primIn p (fun x H => implement_lazy_force x))
+    | tLazy t => EAst.tLambda nAnon (lift 1 0 (implement_lazy_force t))
+    | tForce t => EAst.tApp (implement_lazy_force t) tBox.
   Proof.
     all:try lia.
     all:try apply (In_size); tea.
@@ -69,11 +68,11 @@ Section implement_thunk.
   End Def.
 
   #[universes(polymorphic)]
-  Hint Rewrite @map_primIn_spec @map_InP_spec : implement_thunk.
+  Hint Rewrite @map_primIn_spec @map_InP_spec : implement_lazy_force.
 
   Arguments eqb : simpl never.
 
-  Opaque implement_thunk.
+  Opaque implement_lazy_force.
   Opaque isEtaExp.
   Opaque isEtaExp_unfold_clause_1.
 
@@ -89,18 +88,14 @@ Section implement_thunk.
     now rewrite firstn_skipn.
   Qed.
 
-  Lemma closed_implement_thunk t k : closedn k t -> closedn k (implement_thunk t).
+  Lemma closed_implement_lazy_force t k : closedn k t -> closedn k (implement_lazy_force t).
   Proof using Type.
-    funelim (implement_thunk t); simp implement_thunk; toAll; simpl;
+    funelim (implement_lazy_force t); simp implement_lazy_force; toAll; simpl;
     intros; try easy;
     rewrite -> ?map_map_compose, ?compose_on_snd, ?compose_map_def, ?length_map;
     unfold test_def in *;
     simpl closed in *;
       try solve [simpl; subst; simpl closed; f_equal; auto; rtoProp; solve_all; solve_all]; try easy.
-    - rtoProp. split. eauto.
-      solve_all.
-      replace (#|x.1| + S k) with (#|x.1| + k + 1) by lia.
-      eapply closedn_lift. eauto.
     - solve [simpl; subst; simpl closed; f_equal; auto; rtoProp; solve_all; solve_all_k 6]; try easy.
     - replace (S k) with (k + 1) by lia.
       eapply closedn_lift. eauto.
@@ -109,23 +104,21 @@ Section implement_thunk.
   Hint Rewrite @forallb_InP_spec : isEtaExp.
   Transparent isEtaExp_unfold_clause_1.
 
-  Lemma implement_thunk_lift a k b :
-    implement_thunk (lift a k b) = lift a k (implement_thunk b).
+  Lemma implement_lazy_force_lift a k b :
+    implement_lazy_force (lift a k b) = lift a k (implement_lazy_force b).
   Proof.
     revert k.
-    funelim (implement_thunk b); intros k; cbn; simp implement_thunk; try easy.
+    funelim (implement_lazy_force b); intros k; cbn; simp implement_lazy_force; try easy.
     - destruct (Nat.leb_spec k i); reflexivity.
     - f_equal. rewrite !map_map_compose. solve_all.
       eapply In_All. eauto.
     - cbn. f_equal. rewrite !map_map. solve_all.
       eapply In_All. intros. eapply H; eauto.
-    - cbn. do 2 f_equal. 1: eauto.
+    - cbn. do 1 f_equal. 1: eauto.
       rewrite !map_map. solve_all.
       eapply In_All. intros ? ?. unfold map_def. cbn. f_equal.
       replace (#|x.1| + S k) with (S (#|x.1| + k)) by lia.
       erewrite H; eauto.
-      rewrite permute_lift. lia.
-      f_equal. lia.
     - cbn. f_equal. rewrite !map_map. solve_all.
       eapply In_All. intros ? ?. unfold map_def. cbn. f_equal. erewrite H; eauto.
     - cbn. f_equal. rewrite !map_map. solve_all.
@@ -134,16 +127,16 @@ Section implement_thunk.
     - replace (S k) with (k + 1) by lia. now rewrite <- permute_lift. 
   Qed.
 
-  (* Lemma implement_thunk_subst a k b : *)
-  (*   implement_thunk (subst a k b) = subst (map implement_thunk a) k (implement_thunk b). *)
+  (* Lemma implement_lazy_force_subst a k b : *)
+  (*   implement_lazy_force (subst a k b) = subst (map implement_lazy_force a) k (implement_lazy_force b). *)
   (* Proof using Type. *)
   (*   revert k. *)
-  (*   funelim (implement_thunk b); intros k; cbn; simp implement_thunk; try easy. *)
+  (*   funelim (implement_lazy_force b); intros k; cbn; simp implement_lazy_force; try easy. *)
   (*   all: try now (cbn; f_equal; eauto). *)
   (*   - destruct (Nat.leb_spec k i). *)
   (*     + erewrite nth_error_map. *)
   (*       destruct nth_error; cbn. *)
-  (*       * now rewrite implement_thunk_lift. *)
+  (*       * now rewrite implement_lazy_force_lift. *)
   (*       * len. *)
   (*     + reflexivity. *)
   (*   - f_equal. rewrite !map_map_compose. solve_all. *)
@@ -165,27 +158,25 @@ Section implement_thunk.
   (*     f_equal. now rewrite length_map. *)
   (* Qed. *)
 
-  Lemma implement_thunk_csubst a k b :
+  Lemma implement_lazy_force_csubst a k b :
     closed a ->
-    implement_thunk (ECSubst.csubst a k b) = ECSubst.csubst (implement_thunk a) k (implement_thunk b).
+    implement_lazy_force (ECSubst.csubst a k b) = ECSubst.csubst (implement_lazy_force a) k (implement_lazy_force b).
   Proof using Type.
     intros Ha.
     revert k.
-    funelim (implement_thunk b); intros k; cbn; simp implement_thunk; try easy.
+    funelim (implement_lazy_force b); intros k; cbn; simp implement_lazy_force; try easy.
     all: try now (cbn; f_equal; eauto).
     - destruct Nat.compare => //.
     - f_equal. rewrite !map_map_compose. solve_all.
       eapply In_All. eauto.
     - cbn. f_equal. rewrite !map_map. solve_all.
       eapply In_All. intros. eapply H; eauto.
-    - cbn. do 2 f_equal. 1: eauto.
+    - cbn. do 1 f_equal. 1: eauto.
       rewrite !map_map. solve_all.
       eapply In_All. intros ? ?. unfold map_def. cbn. f_equal.
       setoid_rewrite -> closed_subst at 2.
-      replace (#|x.1| + S k) with ((#|x.1| + k) + 1) by lia.
-      rewrite <- commut_lift_subst_rec. 2: lia.
       rewrite <- closed_subst.
-      2, 3: eapply closed_implement_thunk; eauto.
+      2, 3: eapply closed_implement_lazy_force; eauto.
       f_equal.
       eapply H; eauto.
     - cbn. f_equal. rewrite !map_map. solve_all.
@@ -197,103 +188,103 @@ Section implement_thunk.
       replace (S k) with (k + 1) by lia.
       rewrite <- commut_lift_subst_rec. 2: lia.
       rewrite <- closed_subst.
-      2, 3: eapply closed_implement_thunk; eauto.
+      2, 3: eapply closed_implement_lazy_force; eauto.
       f_equal.
       now rewrite H.
   Qed.
 
-  Lemma implement_thunk_substl s t :
+  Lemma implement_lazy_force_substl s t :
     All (fun x => closed x) s ->
-    implement_thunk (substl s t) = substl (map implement_thunk s) (implement_thunk t).
+    implement_lazy_force (substl s t) = substl (map implement_lazy_force s) (implement_lazy_force t).
   Proof using Type.
     induction s in t |- *; simpl; auto; intros Hall.
     inversion Hall.
     rewrite IHs //.
-    now rewrite implement_thunk_csubst.
+    now rewrite implement_lazy_force_csubst.
   Qed.
 
-  Lemma implement_thunk_iota_red pars args br :
+  Lemma implement_lazy_force_iota_red pars args br :
     All (fun x => closed x) args ->
-    implement_thunk (EGlobalEnv.iota_red pars args br) = EGlobalEnv.iota_red pars (map implement_thunk args) (on_snd implement_thunk br).
+    implement_lazy_force (EGlobalEnv.iota_red pars args br) = EGlobalEnv.iota_red pars (map implement_lazy_force args) (on_snd implement_lazy_force br).
   Proof using Type.
     intros Hall.
     unfold EGlobalEnv.iota_red.
-    rewrite implement_thunk_substl //.
+    rewrite implement_lazy_force_substl //.
     solve_all. now eapply All_skipn.
     now rewrite map_rev map_skipn.
   Qed.
 
-  Lemma implement_thunk_fix_subst mfix : EGlobalEnv.fix_subst (map (map_def implement_thunk) mfix) = map implement_thunk (EGlobalEnv.fix_subst mfix).
+  Lemma implement_lazy_force_fix_subst mfix : EGlobalEnv.fix_subst (map (map_def implement_lazy_force) mfix) = map implement_lazy_force (EGlobalEnv.fix_subst mfix).
   Proof using Type.
     unfold EGlobalEnv.fix_subst.
     rewrite length_map.
     generalize #|mfix|.
     induction n; simpl; auto.
-    f_equal; auto. now simp implement_thunk.
+    f_equal; auto. now simp implement_lazy_force.
   Qed.
 
-  Lemma implement_thunk_cofix_subst mfix : EGlobalEnv.cofix_subst (map (map_def implement_thunk) mfix) = map implement_thunk (EGlobalEnv.cofix_subst mfix).
+  Lemma implement_lazy_force_cofix_subst mfix : EGlobalEnv.cofix_subst (map (map_def implement_lazy_force) mfix) = map implement_lazy_force (EGlobalEnv.cofix_subst mfix).
   Proof using Type.
     unfold EGlobalEnv.cofix_subst.
     rewrite length_map.
     generalize #|mfix|.
     induction n; simpl; auto.
-    f_equal; auto. now simp implement_thunk.
+    f_equal; auto. now simp implement_lazy_force.
   Qed.
 
-  Lemma implement_thunk_cunfold_fix mfix idx n f :
+  Lemma implement_lazy_force_cunfold_fix mfix idx n f :
     All (λ x : term, closed x) (fix_subst mfix) ->
     cunfold_fix mfix idx = Some (n, f) ->
-    cunfold_fix (map (map_def implement_thunk) mfix) idx = Some (n, implement_thunk f).
+    cunfold_fix (map (map_def implement_lazy_force) mfix) idx = Some (n, implement_lazy_force f).
   Proof using Type.
     intros Hcl.
     unfold cunfold_fix.
     rewrite nth_error_map.
     destruct nth_error eqn:heq.
     intros [= <- <-] => /=. f_equal. f_equal.
-    rewrite implement_thunk_substl //. 2:congruence.
-    f_equal. f_equal. apply implement_thunk_fix_subst.
+    rewrite implement_lazy_force_substl //. 2:congruence.
+    f_equal. f_equal. apply implement_lazy_force_fix_subst.
   Qed.
 
-  Lemma implement_thunk_cunfold_cofix mfix idx n f :
+  Lemma implement_lazy_force_cunfold_cofix mfix idx n f :
     All (λ x : term, closed x) (cofix_subst mfix) ->
     cunfold_cofix mfix idx = Some (n, f) ->
-    cunfold_cofix (map (map_def implement_thunk) mfix) idx = Some (n, implement_thunk f).
+    cunfold_cofix (map (map_def implement_lazy_force) mfix) idx = Some (n, implement_lazy_force f).
   Proof using Type.
     intros Hcl.
     unfold cunfold_cofix.
     rewrite nth_error_map.
     destruct nth_error eqn:heq.
     intros [= <- <-] => /=. f_equal.
-    rewrite implement_thunk_substl //. 2:congruence.
-    f_equal. f_equal. apply implement_thunk_cofix_subst.
+    rewrite implement_lazy_force_substl //. 2:congruence.
+    f_equal. f_equal. apply implement_lazy_force_cofix_subst.
   Qed.
 
-  Lemma implement_thunk_nth {n l d} :
-    implement_thunk (nth n l d) = nth n (map implement_thunk l) (implement_thunk d).
+  Lemma implement_lazy_force_nth {n l d} :
+    implement_lazy_force (nth n l d) = nth n (map implement_lazy_force l) (implement_lazy_force d).
   Proof using Type.
     induction l in n |- *; destruct n; simpl; auto.
   Qed.
 
-End implement_thunk.
+End implement_lazy_force.
 
 #[universes(polymorphic)]
-Global Hint Rewrite @map_primIn_spec @map_InP_spec : implement_thunk.
+Global Hint Rewrite @map_primIn_spec @map_InP_spec : implement_lazy_force.
 
-Definition implement_thunk_constant_decl cb :=
-  {| cst_body := option_map implement_thunk cb.(cst_body) |}.
+Definition implement_lazy_force_constant_decl cb :=
+  {| cst_body := option_map implement_lazy_force cb.(cst_body) |}.
 
-Definition implement_thunk_decl d :=
+Definition implement_lazy_force_decl d :=
   match d with
-  | ConstantDecl cb => ConstantDecl (implement_thunk_constant_decl cb)
+  | ConstantDecl cb => ConstantDecl (implement_lazy_force_constant_decl cb)
   | InductiveDecl idecl => InductiveDecl idecl
   end.
 
-Definition implement_thunk_env (Σ : global_declarations) :=
-  map (on_snd (implement_thunk_decl)) Σ.
+Definition implement_lazy_force_env (Σ : global_declarations) :=
+  map (on_snd (implement_lazy_force_decl)) Σ.
 
-Definition implement_thunk_program (p : eprogram) :=
-  (implement_thunk_env p.1, implement_thunk p.2).
+Definition implement_lazy_force_program (p : eprogram) :=
+  (implement_lazy_force_env p.1, implement_lazy_force p.2).
 
 Definition block_wcbv_flags :=
   {| with_prop_case := false ; with_guarded_fix := false ; with_constructor_as_block := true |}.
@@ -377,82 +368,92 @@ Proof.
   eauto.
 Qed.
 
-(* this is false! *)
-(* Lemma implement_thunk_isConstructApp {efl : EEnvFlags} {Σ : global_declarations} t : *)
-(*   isConstructApp (implement_thunk t) = isConstructApp t. *)
-(* Proof. *)
-(*   induction t; try now cbn; eauto. *)
-(*   simp implement_thunk. *)
-(*   rewrite (isConstructApp_mkApps _ [t2]). *)
-(*   rewrite (isConstructApp_mkApps _ [_]). eauto. *)
-(*   simp implement_thunk. *)
-(*   rewrite (isConstructApp_mkApps _ [tBox]). *)
-(*   rewrite IHt. cbn. *)
-(*   rewrite (isConstructApp_mkApps _ [_]). eauto. *)
-(*   simp implement_thunk. *)  
-(*   cbn. *)
-(* Qed. *)
+Lemma implement_lazy_force_isConstructApp {efl : EEnvFlags} t :
+  ~ (exists t', head t = tForce t') ->
+  isConstructApp (implement_lazy_force t) -> isConstructApp t.
+Proof.
+  intros Ht. 
+  induction t; try now cbn; eauto.
+  + simp implement_lazy_force. rewrite !(isConstructApp_mkApps _ [_]).
+    intros. eapply IHt1; eauto. rewrite head_tApp in Ht.
+    firstorder.
+  + simp implement_lazy_force. rewrite !(isConstructApp_mkApps _ [_]).
+    intros. destruct Ht. eexists t. cbn. reflexivity.
+Qed.
 
-(* Lemma implement_thunk_isPrimApp {efl : EEnvFlags} {Σ : global_declarations} t : *)
-(*   isPrimApp (implement_thunk t) = isPrimApp t. *)
+Lemma implement_lazy_force_isPrimApp {efl : EEnvFlags} t :
+  ~ (exists t', head t = tForce t') ->
+  isPrimApp (implement_lazy_force t) -> isPrimApp t.
+Proof.
+  intros Ht. 
+  induction t; try now cbn; eauto.
+  + simp implement_lazy_force. rewrite !(isPrimApp_mkApps _ [_]).
+    intros. eapply IHt1; eauto. rewrite head_tApp in Ht.
+    firstorder.
+  + simp implement_lazy_force. rewrite !(isPrimApp_mkApps _ [_]).
+    intros. destruct Ht. eexists t. cbn. reflexivity.
+Qed.
+
+(* Lemma implement_lazy_force_isPrimApp {efl : EEnvFlags} {Σ : global_declarations} t : *)
+(*   isPrimAppd (implement_lazy_force t) = isPrimApp t. *)
 (* Proof. *)
 (*   induction t; try now cbn; eauto. *)
-(*   simp implement_thunk. *)
+(*   simp implement_lazy_force. *)
 (*   rewrite (isPrimApp_mkApps _ [t2]). *)
 (*   rewrite (isPrimApp_mkApps _ [_]). eauto. *)
 (* Qed. *)
 
-(* Lemma implement_thunk_isLazyApp {efl : EEnvFlags} {Σ : global_declarations} t : *)
-(*   isLazyApp (implement_thunk t) = isLazyApp t. *)
+(* Lemma implement_lazy_force_isLazyApp {efl : EEnvFlags} {Σ : global_declarations} t : *)
+(*   isLazyApp (implement_lazy_force t) = isLazyApp t. *)
 (* Proof. *)
 (*   induction t; try now cbn; eauto. *)
-(*   simp implement_thunk. *)
+(*   simp implement_lazy_force. *)
 (*   rewrite (isLazyApp_mkApps _ [t2]). *)
 (*   rewrite (isLazyApp_mkApps _ [_]). eauto. *)
 (* Qed. *)
 
-Lemma lookup_env_implement_thunk {Σ : global_declarations} kn :
-  lookup_env (implement_thunk_env Σ) kn =
-  option_map (implement_thunk_decl) (lookup_env Σ kn).
+Lemma lookup_env_implement_lazy_force {Σ : global_declarations} kn :
+  lookup_env (implement_lazy_force_env Σ) kn =
+  option_map (implement_lazy_force_decl) (lookup_env Σ kn).
 Proof.
-  unfold implement_thunk_env.
+  unfold implement_lazy_force_env.
   induction Σ at 1 2; simpl; auto.
   case: eqb_spec => //.
 Qed.
 
-Lemma implement_thunk_declared_constant {Σ : global_declarations} c decl :
+Lemma implement_lazy_force_declared_constant {Σ : global_declarations} c decl :
    declared_constant Σ c decl ->
-   declared_constant (implement_thunk_env Σ) c (implement_thunk_constant_decl decl).
+   declared_constant (implement_lazy_force_env Σ) c (implement_lazy_force_constant_decl decl).
 Proof.
   intros H. red in H; red.
-  rewrite lookup_env_implement_thunk H //.
+  rewrite lookup_env_implement_lazy_force H //.
 Qed.
 
-Lemma lookup_constructor_implement_thunk Σ ind c :
-  lookup_constructor (implement_thunk_env Σ) ind c =
+Lemma lookup_constructor_implement_lazy_force Σ ind c :
+  lookup_constructor (implement_lazy_force_env Σ) ind c =
   lookup_constructor Σ ind c.
 Proof.
   unfold lookup_constructor, lookup_inductive, lookup_minductive in *.
-  rewrite lookup_env_implement_thunk.
+  rewrite lookup_env_implement_lazy_force.
   destruct lookup_env as [ [] | ]; cbn; congruence.
 Qed.
 
-Lemma lookup_inductive_implement_thunk Σ ind :
-  lookup_inductive (implement_thunk_env Σ) ind =
+Lemma lookup_inductive_implement_lazy_force Σ ind :
+  lookup_inductive (implement_lazy_force_env Σ) ind =
   lookup_inductive Σ ind.
 Proof.
   unfold lookup_constructor, lookup_inductive, lookup_minductive in *.
-  rewrite lookup_env_implement_thunk.
+  rewrite lookup_env_implement_lazy_force.
   destruct lookup_env as [ [] | ]; cbn; congruence.
 Qed.
 
-Lemma lookup_constructor_pars_args_implement_thunk {efl : EEnvFlags} {Σ ind n} :
-  lookup_constructor_pars_args (implement_thunk_env Σ) ind n = lookup_constructor_pars_args Σ ind n.
+Lemma lookup_constructor_pars_args_implement_lazy_force {efl : EEnvFlags} {Σ ind n} :
+  lookup_constructor_pars_args (implement_lazy_force_env Σ) ind n = lookup_constructor_pars_args Σ ind n.
 Proof.
-  cbn -[lookup_constructor]. now rewrite lookup_constructor_implement_thunk.
+  cbn -[lookup_constructor]. now rewrite lookup_constructor_implement_lazy_force.
 Qed.
 
-Lemma isLambda_implement_thunk c : isLambda c -> isLambda (implement_thunk c).
+Lemma isLambda_implement_lazy_force c : isLambda c -> isLambda (implement_lazy_force c).
 Proof. destruct c => //. Qed.
 
 Definition disable_thunk_term_flags (et : ETermFlags) :=
@@ -477,30 +478,28 @@ Definition switch_off_thunk (efl : EEnvFlags) :=
   {|  has_axioms := efl.(has_axioms) ; has_cstr_params := efl.(has_cstr_params) ; term_switches := disable_thunk_term_flags efl.(term_switches) ; cstr_as_blocks := efl.(cstr_as_blocks) |}.
 
 Lemma transform_wellformed' {efl : EEnvFlags} {Σ : list (kername × global_decl)} n t :
-  has_tApp -> has_tLetIn -> has_tBox ->
+  has_tApp -> has_tBox ->
   wf_glob Σ ->
   @wellformed efl Σ n t ->
-  @wellformed (switch_off_thunk efl) (implement_thunk_env Σ) n (implement_thunk t).
+  @wellformed (switch_off_thunk efl) (implement_lazy_force_env Σ) n (implement_lazy_force t).
 Proof.
-  intros hasa hasl hasbox.
-  revert n. funelim (implement_thunk t); simp_eta; cbn -[implement_thunk
+  intros hasa hasbox.
+  revert n. funelim (implement_lazy_force t); simp_eta; cbn -[implement_lazy_force
     lookup_inductive lookup_constructor lookup_constructor_pars_args
     GlobalContextMap.lookup_constructor_pars_args isEtaExp]; intros m Hwf Hw; rtoProp; try split; eauto.
   all: rewrite ?map_InP_spec; toAll; eauto; try now solve_all.
-  - rewrite lookup_env_implement_thunk. destruct (lookup_env Σ n) => //. destruct g => //=.
+  - rewrite lookup_env_implement_lazy_force. destruct (lookup_env Σ n) => //. destruct g => //=.
     destruct (cst_body c) => //=.
   - unfold lookup_constructor_pars_args in *.
-    rewrite lookup_constructor_implement_thunk. rewrite H2. intuition auto.
-  - rewrite lookup_constructor_pars_args_implement_thunk. len.
+    rewrite lookup_constructor_implement_lazy_force. rewrite H2. intuition auto.
+  - rewrite lookup_constructor_pars_args_implement_lazy_force. len.
     all: destruct cstr_as_blocks; rtoProp; try split; eauto.
     + solve_all.
     + destruct block_args; cbn in *; eauto.
-  - rewrite /wf_brs; cbn -[lookup_inductive implement_thunk].
-    rewrite lookup_inductive_implement_thunk. intuition auto. solve_all. solve_all.
-    replace (#|x.1| + S m) with ((#|x.1| + m) + 1) by lia.
-    eapply wellformed_lift. eauto.
-  - rewrite lookup_constructor_implement_thunk. intuition auto.
-  - unfold wf_fix in *. rtoProp. solve_all. solve_all. now eapply isLambda_implement_thunk.
+  - rewrite /wf_brs; cbn -[lookup_inductive implement_lazy_force].
+    rewrite lookup_inductive_implement_lazy_force. intuition auto. solve_all. solve_all.
+  - rewrite lookup_constructor_implement_lazy_force. intuition auto.
+  - unfold wf_fix in *. rtoProp. solve_all. solve_all. now eapply isLambda_implement_lazy_force.
   - unfold wf_fix in *. rtoProp. solve_all. len. solve_all.
   - unfold wf_fix in *. len. solve_all. rtoProp; intuition auto.
     solve_all.
@@ -510,10 +509,10 @@ Proof.
 Qed.
 
 Lemma transform_wellformed_decl' {efl : EEnvFlags} {Σ : global_declarations} d :
-  has_tApp -> has_tLetIn -> has_tBox ->
+  has_tApp -> has_tBox ->
   wf_glob Σ ->
   @wf_global_decl efl Σ d ->
-  @wf_global_decl (switch_off_thunk efl) (implement_thunk_env Σ) (implement_thunk_decl d).
+  @wf_global_decl (switch_off_thunk efl) (implement_lazy_force_env Σ) (implement_lazy_force_decl d).
 Proof.
   intros.
   destruct d => //=. cbn.
@@ -528,11 +527,11 @@ Proof.
   induction 1; cbn; constructor; auto.
 Qed.
 
-Lemma implement_thunk_env_wf_glob {efl : EEnvFlags} {Σ : global_declarations} :
-  has_tApp -> has_tLetIn -> has_tBox ->
-  wf_glob (efl := efl) Σ -> wf_glob (efl := switch_off_thunk efl) (implement_thunk_env Σ).
+Lemma implement_lazy_force_env_wf_glob {efl : EEnvFlags} {Σ : global_declarations} :
+  has_tApp -> has_tBox ->
+  wf_glob (efl := efl) Σ -> wf_glob (efl := switch_off_thunk efl) (implement_lazy_force_env Σ).
 Proof.
-  intros hasapp haslet hasbox wfg.
+  intros hasapp hasbox wfg.
   assert (extends_prefix Σ Σ). now exists [].
   revert H wfg. generalize Σ at 2 3.
   induction Σ; cbn; constructor; auto.
@@ -547,12 +546,12 @@ Qed.
 
 From MetaCoq.Erasure Require Import EGenericGlobalMap.
 
-Lemma implement_thunk_env_extends {efl : EEnvFlags} {Σ Σ' : global_declarations} :
+Lemma implement_lazy_force_env_extends {efl : EEnvFlags} {Σ Σ' : global_declarations} :
   has_tApp ->
   extends Σ Σ' ->
   wf_glob Σ ->
   wf_glob Σ' ->
-  extends (implement_thunk_env Σ) (implement_thunk_env Σ').
+  extends (implement_lazy_force_env Σ) (implement_lazy_force_env Σ').
 Proof.
   intros hast ext wf wf'.
   intros kn d.
@@ -562,7 +561,7 @@ Proof.
   rewrite (ext g) => //.
 Qed.
 
-Transparent implement_thunk.
+Transparent implement_lazy_force.
 
 Lemma fst_decompose_app_rec t l : fst (decompose_app_rec t l) = fst (decompose_app t).
 Proof.
@@ -577,15 +576,52 @@ Proof. reflexivity. Qed.
 
 Require Import EWcbvEvalCstrsAsBlocksInd.
 
-Lemma implement_thunk_mkApps f args :
-  implement_thunk (mkApps f args) = mkApps (implement_thunk f) (map implement_thunk args).
+Lemma implement_lazy_force_mkApps f args :
+  implement_lazy_force (mkApps f args) = mkApps (implement_lazy_force f) (map implement_lazy_force args).
 Proof.
-  induction args in f |- *; simp implement_thunk.
+  induction args in f |- *; simp implement_lazy_force.
   - reflexivity.
-  - rewrite IHargs. now simp implement_thunk.
+  - rewrite IHargs. now simp implement_lazy_force.
 Qed.
 
-Lemma implement_thunk_eval {efl : EEnvFlags} (fl := block_wcbv_flags) :
+Lemma eval_app_cong_tApp (fl := block_wcbv_flags) Σ t v args res :
+  eval Σ t v ->
+  eval Σ (tApp v args) res ->
+  eval Σ (tApp t args) res.
+Proof.
+  intros. depind H0.
+  - econstructor; eauto. eapply eval_trans; eauto.
+  - econstructor; eauto. eapply eval_trans; eauto.
+  - eapply eval_fix; eauto. eapply eval_trans; eauto.
+  - eapply eval_fix_value; eauto. eapply eval_trans; eauto.
+  - eapply eval_fix'; eauto. eapply eval_trans; eauto.
+  - eapply eval_construct; eauto. eapply eval_trans; eauto.
+  - eapply eval_app_cong; eauto. eapply eval_trans; eauto.
+  - cbn in i. easy.
+Qed.
+
+Lemma eval_app_cong_tApp' (fl := block_wcbv_flags) Σ t arg arg' res :
+  value Σ t ->
+  eval Σ arg arg' ->
+  eval Σ (tApp t arg') res ->
+  eval Σ (tApp t arg) res.
+Proof.
+  intros X H H0. depind H0.
+  - eapply eval_app_cong_tApp; tea. econstructor. constructor. constructor. exact H.
+  - pose proof (eval_trans' H H0_0). subst a'. econstructor; tea.
+  - pose proof (eval_trans' H H0_0). subst av. eapply eval_fix; tea.
+  - pose proof (eval_trans' H H0_0). subst av. eapply eval_fix_value; tea.
+  - eapply value_final in X. pose proof (eval_trans' X H0_). subst f7.
+    pose proof (eval_trans' H H0_0). subst av.
+    eapply eval_fix'; tea.
+  - eapply eval_construct; tea.
+    eapply eval_trans; tea.
+  - eapply eval_app_cong; tea.
+    eapply eval_trans; tea.
+  - now cbn in i.
+Qed.
+
+Lemma implement_lazy_force_eval {efl : EEnvFlags} (fl := block_wcbv_flags) :
   with_constructor_as_block = true ->
   has_cstr_params = false ->
   has_tApp ->
@@ -595,7 +631,7 @@ Lemma implement_thunk_eval {efl : EEnvFlags} (fl := block_wcbv_flags) :
   forall t t',
   @wellformed efl Σ 0 t ->
   EWcbvEval.eval Σ t t' ->
-  @EWcbvEval.eval block_wcbv_flags (implement_thunk_env Σ) (implement_thunk t) (implement_thunk t').
+  @EWcbvEval.eval block_wcbv_flags (implement_lazy_force_env Σ) (implement_lazy_force t) (implement_lazy_force t').
 Proof.
   intros cstrbl prms hasapp hasbox hascofix Σ wfΣ.
   eapply
@@ -604,55 +640,40 @@ Proof.
   { intros. eapply EWcbvEval.eval_wellformed => //; tea. }
   all:intros *.
   - intros; repeat match goal with [H : MCProd.and3 _ _ _ |- _] => destruct H end.
-    simp implement_thunk in *.
+    simp implement_lazy_force in *.
     econstructor; eauto.
   - intros; repeat match goal with [H : MCProd.and3 _ _ _ |- _] => destruct H end.
-    simp implement_thunk in *.
+    simp implement_lazy_force in *.
     econstructor; eauto.
-    now rewrite -implement_thunk_csubst.
+    now rewrite -implement_lazy_force_csubst.
   - intros; repeat match goal with [H : MCProd.and3 _ _ _ |- _] => destruct H end.
-    simp implement_thunk in *.
+    simp implement_lazy_force in *.
     econstructor; eauto.
-    now rewrite -implement_thunk_csubst.
+    now rewrite -implement_lazy_force_csubst.
   - intros; repeat match goal with [H : MCProd.and3 _ _ _ |- _] => destruct H end.
-    simp implement_thunk in *.
+    simp implement_lazy_force in *.
     assert (pars = 0) as -> by now (eapply constructor_isprop_pars_decl_params; eauto).
     pose proof (Hcon := H1).
     rewrite /constructor_isprop_pars_decl in H1.
     destruct lookup_constructor as [[[]] | ] eqn:eqc; cbn in H1; invs H1.
-    eapply eval_zeta => //.
-    1: eauto. rewrite H8.
-    cbn [csubst Nat.compare].
     eapply eval_iota_block => //.
-    + eapply value_final. eapply eval_to_value; eauto.
+    + eauto. 
     + unfold constructor_isprop_pars_decl.
-      rewrite lookup_constructor_implement_thunk. cbn [fst].
-      rewrite eqc //= H7 //. rewrite H8.
-      reflexivity.
-    + rewrite map_map.
-      rewrite nth_error_map H2; eauto.
+      rewrite lookup_constructor_implement_lazy_force. cbn [fst].
+      rewrite eqc //= H7 //. 
+    + rewrite nth_error_map H2; eauto.
       reflexivity.
     + len.
-    + len.
-    +
-      cbn [csubst].
-      cbn [fst snd].
-      rewrite closed_subst.
-      { eapply wellformed_closed in i2.
-        cbn in i2 |- *. solve_all.
-        now eapply closed_implement_thunk.
-      }
-      rewrite Nat.add_0_r.
-      rewrite simpl_subst_k. reflexivity.
-      rewrite -implement_thunk_iota_red.
-      2: eauto.
+    + rewrite H8. len.
+    + rewrite -implement_lazy_force_iota_red.
       eapply wellformed_closed in i2.
       cbn in i2.
       solve_all.
+      rewrite H8. eauto.
   - intros; repeat match goal with [H : MCProd.and3 _ _ _ |- _] => destruct H end.
-    simp implement_thunk in *.
+    simp implement_lazy_force in *.
     eapply eval_fix' => //; eauto.
-    eapply implement_thunk_cunfold_fix.
+    eapply implement_lazy_force_cunfold_fix.
     eapply forallb_All. eapply closed_fix_subst.
     eapply wellformed_closed in i4.
     now cbn in i4. eauto.
@@ -663,13 +684,13 @@ Proof.
     rewrite wellformed_mkApps in i2. eauto.
     cbn in i2. rtoProp. congruence.
   - intros; repeat match goal with [H : MCProd.and3 _ _ _ |- _] => destruct H end.
-    simp implement_thunk in *.
+    simp implement_lazy_force in *.
     econstructor.
-    eapply implement_thunk_declared_constant; eauto.
+    eapply implement_lazy_force_declared_constant; eauto.
     destruct decl. cbn in *. now rewrite H0.
     eauto.
   - intros; repeat match goal with [H : MCProd.and3 _ _ _ |- _] => destruct H end.
-    simp implement_thunk in *.
+    simp implement_lazy_force in *.
     unfold constructor_isprop_pars_decl in *.
     destruct lookup_constructor as [[[mdecl idecl] cdecl']|] eqn:hc => //.
     noconf H2.
@@ -678,32 +699,65 @@ Proof.
     { eapply wellformed_lookup_constructor_pars; tea. }
     eapply eval_proj_block => //; tea. cbn.
     + unfold constructor_isprop_pars_decl.
-      rewrite lookup_constructor_implement_thunk. cbn [fst].
+      rewrite lookup_constructor_implement_lazy_force. cbn [fst].
       rewrite hc //= H1 H7. reflexivity.
     + len.
     + rewrite nth_error_map /=. rewrite H7 in H2; rewrite -H2 in H4; rewrite H4; eauto.
   - intros; repeat match goal with [H : MCProd.and3 _ _ _ |- _] => destruct H end.
-    simp implement_thunk in *.
+    simp implement_lazy_force in *.
     eapply eval_app_cong; eauto.
     revert H1.
     destruct f'; try now cbn; tauto.
-    intros H. cbn in H.
-    (* rewrite implement_thunk_isConstructApp; eauto. *)
-    (* rewrite implement_thunk_isPrimApp; eauto. *)
-    (* rewrite implement_thunk_isLazyApp; eauto. *)
-    all: todo "".
+    { intros H. cbn in H. simp implement_lazy_force.
+      cbn -[implement_lazy_force].
+      rewrite !(isConstructApp_mkApps _ [_]) in H |- *.
+      rewrite !negb_orb in H |- *.
+      rtoProp.
+      assert (¬ ∃ t' : term, head f'1 = tForce t').
+      { eapply eval_to_value in ev as ev'.
+        invs ev'.
+        + inv X. cbn in H4. congruence.
+        + eapply (f_equal head) in H4.
+          rewrite head_mkApps in H4.
+          rewrite (head_mkApps _ [_] )in H4.
+          rewrite <- H4.
+          inv H5.
+          * cbn. congruence. 
+          * cbn. intros []. congruence.
+          * cbn in *. tauto. }
+      repeat split.
+      + eapply PCUICNormal.negb_is_true.
+        intros HH. eapply implement_lazy_force_isConstructApp in HH.
+        apply negbTE in H. congruence.
+        eauto.
+      + rewrite !(isPrimApp_mkApps _ [_]) in H3 |- *.
+        eapply PCUICNormal.negb_is_true.
+        intros HH. eapply implement_lazy_force_isPrimApp in HH.
+        apply negbTE in H3. congruence.
+        eauto.
+      + rewrite (isLazyApp_mkApps _ [_]).
+        clear. induction f'1; simp implement_lazy_force; cbn -[implement_lazy_force]; auto.
+        rewrite (isLazyApp_mkApps _ [_]). eauto.
+        rewrite (isLazyApp_mkApps _ [_]). eauto.
+    }
+    { exfalso.
+      eapply eval_to_value in ev as ev'. cbn in ev'.
+      depelim ev'. inv a0. cbn in H. congruence.
+      destruct args using rev_ind. cbn in H. congruence.
+      rewrite mkApps_app in H. inv H.
+    }
   - intros; repeat match goal with [H : MCProd.and3 _ _ _ |- _] => destruct H end.
-    simp implement_thunk in *.
+    simp implement_lazy_force in *.
     eapply eval_construct_block; tea. eauto.
     2: len; eassumption.
-    rewrite lookup_constructor_implement_thunk; eauto.
+    rewrite lookup_constructor_implement_lazy_force; eauto.
     eapply All2_All2_Set.
     solve_all. now destruct b.
-  - intros wf H; depelim H; simp implement_thunk; repeat constructor.
+  - intros wf H; depelim H; simp implement_lazy_force; repeat constructor.
     destruct a0. eapply All2_over_undep in a. eapply All2_All2_Set, All2_map.
-    cbn -[implement_thunk]. solve_all. now destruct H. now destruct a0.
+    cbn -[implement_lazy_force]. solve_all. now destruct H. now destruct a0.
   - intros evt evt' [] [].
-    simp implement_thunk. simp implement_thunk in e.
+    simp implement_lazy_force. simp implement_lazy_force in e.
     econstructor; eauto.
     setoid_rewrite closed_subst. 2: cbn; auto.
     rewrite simpl_subst_k. reflexivity. auto.
